

Graphene Layer Boundary Condition (Discretized):

$$D_{1\perp} - D_{2\perp} = \sigma \quad (1)$$

$$\mathbf{D} = \varepsilon \mathbf{E} \quad (2)$$

Where ε is the permittivity of the material given by $\kappa\varepsilon_0$ where κ is the dielectric constant of the material and ε_0 is the permittivity of free space. Hence:

$$\varepsilon_1 E_{1\perp} - \varepsilon_2 E_{2\perp} = \sigma \quad (3)$$

Using:

$$\mathbf{E} = -\nabla\phi \quad (4)$$

where $\nabla = \frac{d}{dz}\hat{\mathbf{z}}$ at the boundary, since E_{\parallel} is continuous and hence $\frac{d\phi}{dr} = 0$.

$$\varepsilon_1 \frac{d\phi_1}{dz} - \varepsilon_2 \frac{d\phi_2}{dz} = -\sigma \quad \begin{cases} \phi(z) = \phi_1 & z_b \leq z \leq z_{max} \\ \phi(z) = \phi_2 & z_0 \leq z \leq z_b \end{cases} \quad (5)$$

Discretizing using forward and backward differences for the gradient of $\phi(z)$ above and below the boundary, respectively gives:

$$\frac{d\phi_1}{dz} \approx \frac{\phi_{i,j+1} - \phi_{i,j}}{h} \quad \frac{d\phi_2}{dz} \approx \frac{\phi_{i,j} - \phi_{i,j-1}}{h} \quad (6)$$

where i and j and the r and z indices of the boundary and h is the step size.

Then substituting 6 into equation 5:

$$\begin{aligned} \frac{\varepsilon_1 \phi_{i,j+1} - \varepsilon_1 \phi_{i,j} - \varepsilon_2 \phi_{i,j} + \varepsilon_2 \phi_{i,j-1}}{h} &= -\sigma \\ \varepsilon_1 \phi_{i,j+1} - \varepsilon_1 \phi_{i,j} - \varepsilon_2 \phi_{i,j} + \varepsilon_2 \phi_{i,j-1} &= -h\sigma \\ -(\varepsilon_1 + \varepsilon_2) \phi_{i,j} + \varepsilon_1 \phi_{i,j+1} + \varepsilon_2 \phi_{i,j-1} &= -h\sigma \\ \phi_{i,j} &= \frac{\varepsilon_1 \phi_{i,j+1} + \varepsilon_2 \phi_{i,j-1} + h\sigma}{\varepsilon_1 + \varepsilon_2} \end{aligned} \quad (7)$$

However, σ is dependent on $\phi_{i,j}$:

$$\sigma = \frac{e\phi_{i,j}^2}{\pi\gamma^2} \quad (8)$$

where e is electron charge and γ is the proportionality constant in the dispersion relation:

$$E = \hbar v_F k = \gamma k \quad (9)$$

expressed in units of $eVnm$. Substituting 8 into equation 7 gives a quadratic equation:

$$\phi_{i,j} = \frac{\varepsilon_1 \phi_{i,j+1} + \varepsilon_2 \phi_{i,j-1}}{\varepsilon_1 + \varepsilon_2} + \frac{he}{\pi\gamma^2(\varepsilon_1 + \varepsilon_2)} \phi_{i,j}^2 \quad (10)$$

Using the quadratic formula to give the update equation:

$$\phi_{i,j} = \frac{-b \pm \sqrt{b^2 - 4ac}}{2a} \quad \begin{cases} a = \frac{he}{\pi\gamma^2(\varepsilon_1 + \varepsilon_2)} \\ b = -1 \\ c = \frac{\varepsilon_1 \phi_{i,j+1} + \varepsilon_2 \phi_{i,j-1}}{\varepsilon_1 + \varepsilon_2} \end{cases} \quad (11)$$

but get issues with square root. To get it this to work in the code need:

$$\phi_{i,j} = \frac{-b - \sqrt{|b^2 - 4ac|}}{2a} \quad (12)$$